\documentclass[12pt]{article}
\usepackage[a4paper,margin=1in]{geometry}
\usepackage{graphicx}
\usepackage{setspace}
\usepackage{titling}
\usepackage{ragged2e}
\usepackage{amsmath}
\usepackage{amssymb}
\usepackage{amsfonts}
\usepackage{mathtools} 

\newcommand{\course}{INF8245 — Machine Learning}
\newcommand{\assignment}{Assignment #2}
\newcommand{\university}{Polytechnique Montréal}

\begin{document}

\begin{titlepage}
    \centering
    \vspace*{1.5cm}

    {\LARGE\scshape \university \par}
    \vspace{1.5cm}

    {\Huge\bfseries \course \par}
    \vspace{1cm}

    {\Large\bfseries \assignment \par}
    \vspace{1.5cm}

    {\Huge\bfseries \titletext \par}
    \vspace{2cm}

    {\Large Ali Abbas \textemdash\ Student ID: 2078188 \par}
    \vspace{2cm}

    {\large \supervisor \par}
    \vfill

\end{titlepage}

\cleardoublepage
\pagenumbering{arabic}

\newpage
\section*{Theory: a special case of Stone's theorem}
\label{sec:stone}

\subsection*{Question 4}
\begin{enumerate}
\item[(a)]
Show that for any classifier G, $R(G) = \mathbb{E}[\eta(X)1_{G(X)=0} + (1 - \eta(X))1_{G(X)=1}]$\\ where $\eta(x) = P(g = 1 | X = x)$.\\
\begin{align}
R(G) &= \mathbb{E}_{X, g \thicksim v}[1_{G(X) \neq g}]\nonumber\\
R(G) &= \mathbb{E}[\mathbb{E}[1_{G(X)\neq g} | X]] \:\:\: \text{(Conditional Expectation)}\\\nonumber\\
1_{G(X)\neq g} &= 1_{G(X)=0, g=1} + 1_{G(X)=1, g=0}\nonumber\\
\mathbb{E}[1_{G(X)\neq g} | X = x] &= \mathbb{E}[1_{G(X)=0, g=1} + 1_{G(X)=1, g=0} | X = x]\nonumber\\
&= P(G(X)=0, g=1 | X = x) + P(G(X)=1, g=0 | X = x)\nonumber\\
&= P(g = 1 | X = x)1_{G(X)=0} + P(g = 0 | X = x)1_{G(X)=1}\nonumber\\
&= \eta(x)1_{G(X)=0} + (1 - \eta(x))1_{G(X)=1}\nonumber\\\nonumber\\
R(G) &= \mathbb{E}[\eta(X)1_{G(X)=0} + (1 - \eta(X))1_{G(X)=1}] \:\: \text{(using equation (1))}\nonumber\\\nonumber
\end{align}

\item[(b)]
% \begin{align*}
Show that R^* := R(G^*) = \mathbb{E}[\min(\eta(X), 1 - \eta(X))]\\\\
R^* &= \mathbb{E}[\min(\eta(X), 1 - \eta(X))]\\
R^* &= \mathbb{E}[\eta(X)1_{G^*(X) = 0} + (1 - \eta(X))1_{G^*(X) = 1}]\\\\
% \end{align*}
G^*(X) = \begin{cases}
0 & \text{if } \eta(X) < 1/2\\
1 & \text{elsewhere} 
\end{cases}$\\


Suppose $\eta(X)\ge \tfrac12$, then $\eta(X)\, \mathbf{1}_{G^*(X)=0}=0$\\
and $(1-\eta(X))\, \mathbf{1}_{G^*(X)=1}=1-\eta(X)\le \eta(X)$\\
So, $\min(\eta(X), 1 - \eta(X)) = (1 - \eta(X)) \: and \: R^* = \mathbb{E}[(1 - \eta(X))]$\\\\
Suppose $\eta(X)< \tfrac12$, then $\eta(X)\, \mathbf{1}_{G^*(X)=0}=\eta(X) < 1 - \eta(X)$\\
and $(1-\eta(X))\, \mathbf{1}_{G^*(X)=1}=0$\\
So, $\min(\eta(X), 1 - \eta(X)) = \eta(X) \: and \: R^* = \mathbb{E}[\eta(X)]$\\\\
Thus, in both cases, we have \\ $R^* = \mathbb{E}[\min(\eta(X), 1 - \eta(X))]$\\
\noindent\rule{8cm}{0.4pt}\\\\
Show that for any classifier G, $R(G) - R^* = \mathbb{E}[|2\eta(X) - 1|1_{G(X) \neq G^*(X)}]$\\

$1_{G(X)= 0} = 1 - 1_{G(X)= 1}$ and $1_{G^*(X)= 0} = 1 - 1_{G^*(X)= 1}$\\
$1_{G(X)=0} - 1_{G^*(X)=0} = 1 - 1_{G(X)=1} - 1 + 1_{G^*(X)=1} = 1_{G^*(X)=1} - 1_{G(X)=1}$
\begin{align*}
R(G) - R^* &= \mathbb{E}[|2\eta(X) - 1|1_{G(X) \neq G^*(X)}]\nonumber\\\\
&= \mathbb{E}[\eta(X)1_{G(X)=0} + (1 - \eta(X))1_{G(X)=1}]\\
&- \mathbb{E}[\eta(X)1_{G^*(X)=0} + (1 - \eta(X))1_{G^*(X)=1}]\\\\
&= \mathbb{E}[\eta(X)1_{G(X)=0} - \eta(X)1_{G^*(X)=0} + (1 - \eta(X))1_{G(X)=1}\\
&- (1 - \eta(X))1_{G^*(X)=1}]\\\\
&= \mathbb{E}[\eta(X)(1_{G(X)=0} - 1_{G^*(X)=0}) + (1 - \eta(X))(1_{G(X)=1} - 1_{G^*(X)=1})]\\
&= \mathbb{E}[\eta(X)(1_{G^*(X)=1} - 1_{G(X)=1}) + (1 - \eta(X))(1_{G(X)=1} - 1_{G^*(X)=1})]\\
&= \mathbb{E}[(2\eta(X) - 1)(1_{G^*(X)=1} - 1_{G(X)=1})]\\
\end{align*}

Case 1: suppose $1_{G^*(X) \neq G(X)} = 0$, then $1_{G^*(X)} = 1_{G(X)}$; $1_{G^*(X)} - 1_{G(X)} = 0$\\\\
Case 2: suppose $1_{G^*(X) \neq G(X)} = 1$\\
if $G^*(X) = 1$ and $G(X) = 0$, then G^*(X)=1  \: and \: \eta \geq 1/2$\\
\hookrightarrow 2\eta(X) -1 \geq 0$\\
\hookrightarrow (2\eta(X) - 1 )(1-0) = 2\eta(X) - 1$\\
since \eta(X) \geq 1/2, \: then \: $2\eta(X) - 1 = |2\eta(X) - 1|$\\\\
if $G^*(X) = 0$ and $G(X) = 1$, then G^*(X)=0  \: and \: \eta < 1/2$\\
\hookrightarrow 2\eta(X) -1 < 0$\\
\hookrightarrow (2\eta(X) - 1 )(0-1) = -(2\eta(X) - 1) = 1 - 2\eta(X)$\\
since \eta(X) < 1/2, \: then \: $1 - 2\eta(X) = |2\eta(X) - 1|$\\\\
Thus, in both cases, we have \\ $R(G) - R^* = \mathbb{E}[|2\eta(X) - 1|1_{G(X) \neq G^*(X)}]$\\
% \noindent\rule{8cm}{0.4pt}\\\\
\item[(c)]
Show that ${R}(\hat{G}_n) - R^* \leq 2\mathbb{E}[|\eta(X) - \hat{\eta}_n(X)|]$.
\begin{align*}
R(\hat{G}_{n}) - R^* &= \mathbb{E}[|2\eta(X) - 1|1_{\hat{G}_{n}(X) \neq G^*(X)}]\\
&= 2\mathbb{E}[|\eta(X) - 1/2|1_{\hat{G}_{n}(X) \neq G^*(X)}]\\
	\end{align*}
G^*(X) = \begin{cases}
1 & \text{if } \eta(X) \geq 1/2\\
0 & \text{elsewhere}
\end{cases}$\\

$\hat{G}_{n}(X)$ = \begin{cases}
1 & \text{if } \hat{\eta}_n(X) \geq 1/2\\
0 & \text{elsewhere}
\end{cases}$\\

Case 1: suppose G^*(X) = 1 \: and \: \hat{G}_n(X) = 0$, then $\eta(X) \geq 1/2$ and $\hat{\eta}_n(X) < 1/2$\\
$\hookrightarrow \hat{\eta}_n(X) < 1/2 \leq \eta(X) \rightarrow |\eta(X) - \hat{\eta}_n(X)| \geq |\eta(X) - 1/2|$\\\\
Case 2: suppose \: G^*(X) = 0 \: and \: \hat{G}_n(X) = 1$, then $\eta(X) < 1/2$ and $\hat{\eta}_n(X) \geq 1/2$\\
\hookrightarrow \eta(X) < 1/2 \leq \hat{\eta}_n(X) \rightarrow |\eta(X) - \hat{\eta}_n(X)| \geq |\eta(X) - 1/2|$\\\\
\text{Thus, in both cases, we have} $|\eta(X) - \hat{\eta}_n(X)| \geq |\eta(X) - 1/2|$
\begin{align*}
R(\hat{G}_n) - R^* &= 2\mathbb{E}[|\eta(X) - 1/2|1_{\hat{G}_n(X) \neq G^*(X)}]\\
&\leq 2\mathbb{E}[|\eta(X) - \hat{\eta}_n(X)|1_{\hat{G}_n(X) \neq G^*(X)}]\\
&\leq 2\mathbb{E}[|\eta(X) - \hat{\eta}_n(X)|]\\
\end{align*}


\end{enumerate}
\subsection*{Question 5}
\begin{enumerate}
\item[(a)]
Show that $\mathbb{E}[(\eta(x) - \hat{\eta}_n(X))^2] \leq 2\mathbb{E}[(\eta(x) - \tilde{\eta}_n(X))^2] + 2\mathbb{E}[(\tilde{\eta}_n(x) - \hat{\eta}_n(X))^2]$ 
\begin{align*}
	\eta(x) - \hat{\eta}_n(x) &= \eta(x) - \tilde{\eta}_n(X) + \tilde{\eta}_n(x) - \hat{\eta}_n(x)\\
	 &= (\eta(x) - \tilde{\eta}_n(x)) + (\tilde{\eta}_n(x) - \hat{\eta}_n(x))\\
	 (\eta(x) - \hat{\eta}_n(x))^2 &= (\eta(x) - \tilde{\eta}_n(x))^2 + (\tilde{\eta}_n(x) - \hat{\eta}_n(x))^2 \\
	 &+ 2(\eta(x) - \tilde{\eta}_n(x))(\tilde{\eta}_n(x) - \hat{\eta}_n(x))\\
\end{align*}
(Using $2ab \leq a^2 + b^2$)
\begin{align*}
	 2(\eta(x) - \hat{\eta}_n(x))(\hat{\eta}_n(x) - \tilde{\eta}_n(x)) &\leq (\eta(x) - \tilde{\eta}_n(x))^2 + (\tilde{\eta}_n(x) - \hat{\eta}_n(x))^2 \\
	 2(\mathbb{E}[(\eta(x) - \hat{\eta}_n(X))(\tilde{\eta}_n(X) - \hat{\eta}_n(X))]) &\leq \mathbb{E}[(\eta(x) - \tilde{\eta}_n(X))^2] + \mathbb{E}[(\tilde{\eta}_n(X) - \hat{\eta}_n(X))^2]\\
	 \mathbb{E}[(\eta(x) - \hat{\eta}_n(X))^2] &\leq \mathbb{E}[(\eta(x) - \tilde{\eta}_n(X))^2] + \mathbb{E}[(\tilde{\eta}_n(X) - \hat{\eta}_n(X))^2]\\
	 &+ \mathbb{E}[(\eta(x) - \tilde{\eta}_n(X))^2] + \mathbb{E}[(\tilde{\eta}_n(X) - \hat{\eta}_n(X))^2]\\
	 &= 2\mathbb{E}[(\eta(x) - \tilde{\eta}_n(X))^2] + 2\mathbb{E}[(\tilde{\eta}_n(X) - \hat{\eta}_n(X))^2]\\
	%  \shortintertext{Using 2ab \leq a^2 + b^2}\\
	\end{align*}
\item[(b)] Show that $\mathbb{E}[(\eta(X) - \tilde{\eta}_n(X))^2] \leq \varepsilon^2 + \mathbb{E}\left[\sum_{i=1}^{n} w_{n,i}(X)1_{\|X_i - X\| \geq \delta}\right]$.

\begin{align*}
\eta(X) - \tilde{\eta}_n(X) &= \eta(X) - \sum_{i=1}^n w_{n,i}(X) \eta(X_i)\\
&= \sum_{i=1}^n w_{n,i}(X) \eta(X) - \sum_{i=1}^n w_{n,i}(X) \eta(X_i)\\
&= \sum_{i=1}^n w_{n,i}(X)(\eta(X) - \eta(X_i))
\end{align*}

Since $\sum_{i=1}^n w_{n,i}(X) = 1$, Jensen's inequality gives:

\begin{align*}
(\eta(X) - \tilde{\eta}_n(X))^2 &= \Big(\sum_{i=1}^n w_{n,i}(X)(\eta(X) - \eta(X_i))\Big)^2\\
&\leq \sum_{i=1}^n w_{n,i}(X)(\eta(X) - \eta(X_i))^2\\
\mathbb{E}[(\eta(X) - \tilde{\eta}_n(X))^2] &\leq \mathbb{E}[\sum_{i=1}^n w_{n,i}(X)(\eta(X) - \eta(X_i))^2]
\\
\mathbb{E}[(\eta(X) - \tilde{\eta}_n(X))^2] &\leq \mathbb{E}[\sum_{i=1}^n w_{n,i}(X)(\eta(X) - \eta(X_i))^2 1_{\|X_i - X\| < \delta}]\\
&\quad + \mathbb{E}[\sum_{i=1}^n w_{n,i}(X)(\eta(X) - \eta(X_i))^2 1_{\|X_i - X\| \geq \delta}]
\end{align*}

$(\varepsilon, \delta)$-definition of limit: If $\eta$ is continuous, then for every $\varepsilon > 0$, there exists $\delta > 0$ such that for all $p \in \mathbb{R}^d$:

$\|x - p\| < \delta \Rightarrow |\eta(x) - \eta(p)| < \epsilon$\\

\end{enumerate}

\end{document}